Ported revisions 5651:5659 from HOL to HOL-Omega.
Also removed some comments from Type-sig.sml.

src/0/Type-sig.sml
@@ -5,9 +5,6 @@ sig
  eqtype hol_type
  type tyvar = string * kind * int (* rank *)
 
-(* val mk_clos       : hol_type Subst.subs * hol_type -> hol_type *)
-(* val norm_clos     : hol_type -> hol_type *)
-
  val mk_vartype    : string -> hol_type
  val mk_vartype_opr : tyvar -> hol_type
  val mk_primed_vartype : string -> hol_type
