src/bool/DefnBase.sml
@@ -102,8 +102,9 @@ end;
  ---------------------------------------------------------------------------*)
 
 local open boolTheory
-      val non_datatype_congs = ref [LET_CONG, COND_CONG, IMP_CONG,
-                                    literal_case_CONG]
+      val non_datatype_congs = 
+        ref [LET_CONG, COND_CONG, IMP_CONG, 
+             AND_CONG, OR_CONG, literal_case_CONG]
 in
   fun read_congs() = !non_datatype_congs
   fun write_congs L = (non_datatype_congs := L)
