examples/dev/sw2/regAlloc.sml
@@ -6,8 +6,12 @@ struct
 open HolKernel Parse boolLib bossLib;
 open pairLib pairSyntax PairRules NormalTheory Normal basic;
 
+val atom_tm = prim_mk_const{Name="atom",Thy="Normal"}
+fun mk_atom tm = mk_comb (inst [alpha |-> type_of tm] atom_tm,tm)
+
 (* --------------------------------------------------------------------*)
 (* --------------------------------------------------------------------*)
+
 
 structure M = Binarymap
 structure S = Binaryset
@@ -37,9 +41,9 @@ val numRegs = ref 10;
 
 fun mk_regs() = 
   let 
-    fun f n = if n = !numRegs then [] else mk_var("r" ^ Int.toString(n) , !VarType) :: f(n+1)
-  in
-    f 0
+    fun f n = if n = !numRegs then [] 
+               else mk_var("r" ^ Int.toString(n) , !VarType) :: f(n+1)
+  in f 0
   end
 
 val regL = ref (mk_regs());
@@ -63,7 +67,7 @@ fun tvarOrder (t1:term,t2:term) =
 fun is_fun exp = 
   (* is_var exp andalso *) 
   (#1 (dest_type (type_of exp)) = "fun")
-  handle _ => false;
+  handle HOL_ERR _ => false;
 
 (* --------------------------------------------------------------------*)
 (* make variables                                                      *)
@@ -101,45 +105,41 @@ fun fv exp =
 (* allocate a register or spill a variable *)
 
 fun alloc_one cont regenv x =
-  let val all = !regL (* allregs *) in
-    if is_reg x then Alloc(x) else
-    let 
-      val free = fv cont
-      val live =    (* the set of registers already assigned to the live variables in cont *)
-        List.foldl
-          (fn (y,live) =>
-            if is_reg y then S.add (live,y) else       (* registers that have been used *)
-              S.add (live, M.find (regenv, y))         (* registers (and memory) already assigned *) 
-                handle NotFound => live)
-          (S.empty tvarOrder)
-          free
-      val candidate =  (* the first available register *)
-        List.find
-          (fn r => not (S.member(live,r)))
-          all
-    in
-       case candidate of
-         SOME r => Alloc(r)
-       | NONE => 
-           let val y = valOf (
-              List.find
-              (fn y =>
-                 let val k = M.find(regenv,y) in
-                   not (is_reg y) andalso             (* exclude variables that are in registers *)
-                   not (is_mem k) andalso             (* exclude spilled variables (in memory) *) 
-                  (List.exists (fn z => (k = z)) all) (* made sure that it has been assigned a register *)
-                  end
-                  handle NotFound => false)
-             (List.rev free))
-               val _ = if !DEBUG then 
-                  (print ("register allocation failed for " ^ (term_to_string x) ^ "; ");
-                   print ("spilling " ^ (term_to_string y) ^ " from " ^ (term_to_string (M.find(regenv,y))) ^ "\n"))
-                  else ()
-           in
-             Spill(y)
-           end
+ let val allregs = !regL 
+ in
+ if is_reg x then Alloc(x) else
+ let val free = fv cont
+     val live = (* set of registers already assigned to live var in cont *)
+       List.foldl (fn (y,live) =>
+         if is_reg y then (* registers that have been used *)
+           S.add (live,y) 
+         else (* registers (and memory) already assigned *) 
+           S.add (live, M.find (regenv, y)) handle NotFound => live)
+       (S.empty tvarOrder) free
+      val candidate = List.find (fn r => not (S.member(live,r))) allregs
+                     (* the first available register *)
+ in
+  case candidate 
+   of SOME r => Alloc(r)
+    | NONE => let 
+       fun OK y = 
+         let val k = M.find(regenv,y) 
+         in not(is_reg y) andalso (* exclude vars in registers        *)
+            not(is_mem k) andalso (* exclude spilled vars (in memory) *)
+            Lib.mem k allregs     (* ensure it's assigned a register  *)
+         end handle NotFound => false
+       val y = valOf(List.find OK (List.rev free))
+       val _ = if !DEBUG then 
+                 (print ("register allocation failed for "^
+                         term_to_string x^"; ");
+                  print ("spilling "^term_to_string y^
+                         " from " ^term_to_string (M.find(regenv,y))^"\n"))
+               else ()
+     in
+        Spill(y)
      end
-  end
+ end
+end;
 
 (* --------------------------------------------------------------------*)
 (* For Tuple and Function calls                                        *)
@@ -147,12 +147,13 @@ fun alloc_one cont regenv x =
 (* --------------------------------------------------------------------*)
 
 fun find_pos (regenv,x) =
-  if is_reg x orelse is_word_literal x orelse numSyntax.is_numeral x orelse is_const x then x
-  else
-    let val v = M.find (regenv, x) in
-      if is_reg v orelse is_mem v then v
+ if is_reg x orelse is_word_literal x orelse 
+    numSyntax.is_numeral x orelse is_const x then x
+ else
+   let val v = M.find (regenv, x) 
+   in if is_reg v orelse is_mem v then v 
       else raise (Fail "find_pos...")
-    end 
+   end 
   ;
 
 fun tuple_subst_rules xs regenv =
@@ -164,33 +165,31 @@ fun tuple_subst_rules xs regenv =
       xs;
 
 (* --------------------------------------------------------------------*)
-(* Attempt to allocate registers for a tuple                           *)
+(* Attempt to allocate registers for a tuple.                          *)
 (* If the tuple contains only one variable, we always allocate a       *)
 (* register for it by spilling another variable;                       *)
 (* on the other hand, if the tuple contains several variables, and some*)
 (* of them couldn't be assigned registers, we always spill them into   *)
-(* the memory. (this can be optimized a little)                        *)
+(* the memory (this can be optimized a little).                        *)
 (* --------------------------------------------------------------------*)
 
 fun alloc cont regenv x =
-  if is_pair x then
-    let 
-      val xs = strip_pair x
-      val env =
-        #2(List.foldl 
-          (fn (t, (cont', env')) => 
-	     case alloc_one cont' env' t of 
-	        Alloc(r) => (mk_pair(cont', t), M.insert(env', t, r))           (* assign a register *) 
-              | Spill(n) => (mk_pair(cont',t), M.insert(env', t, next_mvar()))  (* assign a memory slot *)
-	  ) (cont,regenv) xs
-        ) 
-    in
+ if is_pair x then
+  let val xs = strip_pair x
+      val (_,env) = List.foldl (fn (t,(cont',env')) => 
+                 case alloc_one cont' env' t 
+             of Alloc(r) => (* assign a register *) 
+                            (mk_pair(cont', t), M.insert(env', t, r))
+              | Spill(n) => (* assign a memory slot *)
+                   (mk_pair(cont',t), M.insert(env', t, next_mvar()))
+          ) (cont,regenv) xs
+  in
      (Alloc(subst (tuple_subst_rules xs env) x), env)
-    end
-  else            (* single variable *)
-     case alloc_one cont regenv x of 
-	 Alloc(r) => (Alloc(r), M.insert(regenv, x, r))
-      |  Spill(n) => (Spill(n), regenv)
+  end
+  else (* single variable *)
+    case alloc_one cont regenv x 
+     of Alloc(r) => (Alloc(r), M.insert(regenv, x, r))
+      | Spill(n) => (Spill(n), regenv)
   ;
 
 (* --------------------------------------------------------------------*)
@@ -207,15 +206,15 @@ exception NoReg of term
 
 fun find_reg (regenv,x) =
   if is_reg x then x
-  else if is_word_literal x orelse numSyntax.is_numeral x orelse is_const x then x
+  else if is_word_literal x orelse 
+          numSyntax.is_numeral x orelse is_const x then x
   else
-    let val v = M.find (regenv, x) in
-      if is_reg v then v
-      else raise (NoReg x)
+    let val v = M.find (regenv, x) 
+    in if is_reg v then v else raise (NoReg x)
     end
-  handle NotFound => raise (NoReg x)
+  handle NotFound => raise (NoReg x);
 
-fun mk_subst_rules xs regenv =         (* replace variables with registers *)
+fun mk_subst_rules xs regenv = (* replace variables with registers *)
     List.foldl
       (fn (x,ys) =>
         if is_var x then (x |-> find_reg (regenv, x)) :: ys
@@ -226,44 +225,39 @@ fun mk_subst_rules xs regenv =         (* replace variables with registers *)
 (* let x = (let v = M in N) in e2   --> let x = M in let v = N in e2 *)
 
 fun concat e1 x e2 = 
-  if is_let e1 then 
-    let val (v,M,N) = dest_plet e1 in
-        mk_plet (v, M, concat N x e2)
-    end
-  else 
-    mk_plet (x, e1, e2)
+  if is_let e1 
+  then let val (v,M,N) = dest_plet e1 in mk_plet (v, M, concat N x e2) end
+  else mk_plet (x, e1, e2);
 
 (* Add a mapping into the environment *)
 
-fun add x r regenv =
-  if is_reg x then regenv
-  else M.insert(regenv, x, r)
+fun add x r regenv = if is_reg x then regenv else M.insert(regenv, x, r);
 
-fun list_mem x xs =  (*  membership in a list   *)
-  not ((List.find (fn k => (k = x)) xs) = NONE)
 
 (* --------------------------------------------------------------------*)
 (* Spill to memory                                                     *)
-(* Restore from memory                                                  *)
+(* Restore from memory                                                 *)
 (* --------------------------------------------------------------------*)
 
 fun save x exp regenv =
-  let val v = next_mvar()
-      val regenv1 = M.insert(regenv, x, v)    (* x is spilled to memory *)
-      val _ = if !DEBUG then 
-                print ("saving " ^ term_to_string x ^ " to " ^ term_to_string v ^"\n")
-               else ()
-  in 
-     (mk_plet (v, M.find(regenv,x), exp), regenv1)   (* let m[.] = r[.] in exp[m[.]] *)
+ let val v = next_mvar()
+     val regenv1 = M.insert(regenv, x, v)    (* x is spilled to memory *)
+     val _ = if !DEBUG then 
+             print ("saving "^term_to_string x^
+                    " to " ^ term_to_string v ^"\n")
+             else ()
+  in    (* let m[.] = r[.] in exp[m[.]] *)
+    (mk_plet (v, M.find(regenv,x), exp), regenv1)
   end
 
 fun restore x exp regenv =
   let val v = next_tvar ()
       val _ = if !DEBUG then 
-                print ("restoring " ^ term_to_string x ^ " from " ^ term_to_string (M.find(regenv,x)) ^"\n")
+                print ("restoring "^term_to_string x^
+                       " from "^term_to_string (M.find(regenv,x))^"\n")
                else ()
   in mk_plet (v, M.find (regenv,x), 
-          subst_exp [x |-> v] exp)    (* let v = m[.] in exp[x <- v] *)
+              subst_exp [x |-> v] exp)  (* let v = m[.] in exp[x <- v] *)
   end
 
 (* --------------------------------------------------------------------*)
@@ -274,139 +268,129 @@ fun restore x exp regenv =
 (* g' is for allocating registers in expressions *)
 
 fun g' dest cont regenv exp =
-  if is_word_literal exp orelse numSyntax.is_numeral exp orelse is_const exp orelse 
-     is_fun exp orelse is_mem exp then NoSpill (exp, regenv)
-  else if is_var exp then NoSpill (subst (mk_subst_rules [exp] regenv) exp, regenv)
-  else if is_cond exp then
-    let val (c,e1,e2) = dest_cond exp
-        val (cmpop,ds) = strip_comb c
-        val (d0,d1) = (hd ds, hd (tl ds))
-        (*
-        val (ds0,ds1) = (#2 (strip_comb d0), #2 (strip_comb d1))
-        val c' = list_mk_comb (cmpop, [subst (mk_subst_rules ds0 regenv) d0, subst (mk_subst_rules ds1 regenv) d1])
-        *)
-        val c' = list_mk_comb (cmpop, [find_reg(regenv,d0), find_reg(regenv,d1)])
-        fun f e1 e2 = mk_cond(c', e1, e2)
-    in
-        g'_if dest cont regenv exp f e1 e2
-    end
-  else if is_pair exp then
-      NoSpill (subst (tuple_subst_rules (strip_pair exp) regenv) exp, regenv)
-  else if is_let exp then
-       g dest cont regenv exp
-  else if is_comb exp then
-    let val (op0,xs) = strip_comb exp in
-      if is_binop op0 (* includes orelse is_cmpop op0 orelse is_relop op0 *)
-      then
-        NoSpill (subst (mk_subst_rules xs regenv) exp, regenv)
-      else if is_fun op0 then  (* function application *)
-        let val ys = List.foldl (fn (t, ls) => (strip_pair t) @ ls) [] xs
-        in  NoSpill (subst (tuple_subst_rules ys regenv) exp, regenv)
-        end
-      else raise regAlloc
-          ("g': this case hasn't been unimplemented -- " ^ term_to_string exp)
-    end
-  else NoSpill (exp, regenv)
+ if is_word_literal exp orelse numSyntax.is_numeral exp orelse 
+    is_const exp orelse is_fun exp orelse is_mem exp 
+   then NoSpill (exp, regenv) else 
+ if is_var exp 
+    then NoSpill (subst (mk_subst_rules [exp] regenv) exp, regenv) else 
+ if is_cond exp 
+    then let val (c,e1,e2) = dest_cond exp
+             val (cmpop,ds) = strip_comb c
+             val (d0,d1) = (hd ds, hd (tl ds))
+             (* val (ds0,ds1) = (#2 (strip_comb d0), #2 (strip_comb d1))
+                val c' = list_mk_comb 
+                         (cmpop, [subst (mk_subst_rules ds0 regenv) d0, 
+                                  subst (mk_subst_rules ds1 regenv) d1]) 
+             *)
+             val c' = list_mk_comb (cmpop, [find_reg(regenv,d0), 
+                                            find_reg(regenv,d1)])
+             fun f e1 e2 = mk_cond(c', e1, e2)
+         in
+            g'_if dest cont regenv exp f e1 e2
+        end else 
+ if is_pair exp 
+    then NoSpill (subst (tuple_subst_rules (strip_pair exp) regenv) exp, 
+                  regenv) else 
+ if is_let exp 
+    then g dest cont regenv exp else
+ if is_comb exp 
+    then
+      let val (opr,xs) = strip_comb exp 
+      in if is_binop opr (* includes is_cmpop opr orelse is_relop opr *)
+            then NoSpill (subst (mk_subst_rules xs regenv) exp, regenv) else
+         if is_fun opr   (* function application *)
+            then 
+              let val ys = List.foldl (fn (t,ls) => strip_pair t @ ls) [] xs
+              in NoSpill (subst (tuple_subst_rules ys regenv) exp, regenv)
+              end 
+            else raise regAlloc 
+                         ("g': this case hasn't been implemented -- "^
+                          term_to_string exp)
+      end
+ else NoSpill (exp, regenv)
 
 and
 
-(* when g' accesses a spilled variable, a NoReg exception is raised since we cannot find the variable in regenv. 
-   Thus a restore is required, which restores the value of a variable from the memory to a register. *)
+(*---------------------------------------------------------------------------*)
+(* When g' accesses a spilled variable, a NoReg exception is raised since    *)
+(* we cannot find the variable in regenv. Thus a restore is required, which  *)
+(* restores the value of a variable from the memory to a register.           *)
+(*---------------------------------------------------------------------------*)
 
 g'_and_restore dest cont regenv exp =
   g' dest cont regenv exp
-  handle NoReg x =>                              (* x is stored in the memory, need to be assigned a register *)
-      g dest cont regenv (restore x exp regenv)  (* restore the spilled x from the memory *)
+  handle NoReg x (* x is stored in the memory, assign it a register *)
+  => g dest cont regenv (restore x exp regenv)  
+    (* restore the spilled x from the memory *)
 
 and
 
-(* g deals with the let v = ... in ... structure.  *)
+(*---------------------------------------------------------------------------*)
+(* g deals with the let v = ... in ... structure.                            *)
+(*---------------------------------------------------------------------------*)
 
- g dest cont regenv exp = 
-  if is_let exp then                        (*  exp = LET (\v. N) M  *)
-     let
-       val (x,M,N) = dest_plet exp
-       val cont' = mk_pair(N, cont) (* concat N dest cont *)
-     in
-       if is_mem x orelse is_reg x then 
-          case (g x cont regenv N) of
-               ToSpill(e2, ys) =>
-                 ToSpill (exp, ys)
-            |  NoSpill(e2, regenv2) => NoSpill(mk_plet(x,M,e2), regenv2)
-       else
-       case g'_and_restore x cont' regenv M of
-            ToSpill(exp1, ys) => ToSpill(concat exp1 x N, ys)
-         |  NoSpill(exp1, regenv1) =>
-            ( case (alloc cont' regenv1 x) of
-                 (Spill(y), env) => 
-                     let val op_vars = free_vars N
-                     in
-		       (if list_mem y op_vars then
-                         ToSpill (exp, [#1 (valOf(List.find (fn (key,value) =>
-                                          is_reg value andalso not (list_mem key op_vars)) (M.listItems(env))))])
-                       else ToSpill (exp, [y]))
-                       handle _ => ToSpill (exp, [y])
-(*
-		       (if list_mem y op_vars then
-			 ToSpill (exp, [valOf(List.find (fn t => 
-					  is_reg (M.find(regenv1,t)) andalso not (list_mem t op_vars)
-					  handle _ => false) (free_vars cont'))])
-		       else ToSpill (exp, [y]))
-                       handle _ => ToSpill (exp, [y])
-*)
-                     end
-              |  (Alloc(r), env) => 
-		     let val (exp2,env') = g_repeat dest cont env N
-                     in NoSpill(concat exp1 r exp2, env')
-                     end
-(*
-		   (case (g dest cont env N) of
-                     ToSpill(e2, ys) =>
-                       if list_mem x ys then
-                          let val (e',regenv') = save x e2 (add x r regenv1) cont
-                              val x_saved = concat exp1 r e' in
-                            (case List.filter (fn y => y <> x) ys of
-                                  []      => g dest cont regenv' x_saved
-                               |  ys_left => ToSpill(x_saved, ys_left)
-                            )
-                          end
-                       else
-                         ToSpill (mk_plet(x,M,N), ys)
-                      |  NoSpill(e2', regenv2) => NoSpill(concat exp1 r e2', regenv2)
-                   )
-*)
-            )
-     end
-  else
+g dest cont regenv exp = 
+ if not (is_let exp) then 
      g'_and_restore dest cont regenv exp
- 
+ else (*  exp = LET (\v. N) M  *)
+ let val (x,M,N) = dest_plet exp
+     val cont' = mk_pair(N,cont) (* concat N dest cont *)
+ in
+  if is_mem x orelse is_reg x 
+  then case g x cont regenv N
+        of ToSpill(e2,ys) => ToSpill (exp, ys)
+         | NoSpill(e2,regenv2) => NoSpill(mk_plet(x,M,e2),regenv2)
+  else
+    case g'_and_restore x cont' regenv M 
+     of ToSpill(exp1, ys) => ToSpill(concat exp1 x N, ys)
+      | NoSpill(exp1, regenv1) =>
+          case (alloc cont' regenv1 x) 
+           of (Spill(y), env) => 
+                let val op_vars = free_vars N
+                in (if Lib.mem y op_vars then 
+                      let val opt = 
+                            List.find (fn (key,value) =>
+                                        is_reg value andalso 
+                                        not (Lib.mem key op_vars))
+                                      (M.listItems env)
+                          val (thing,_) = valOf opt
+                      in
+                        ToSpill (exp, [thing])
+                      end
+                    else ToSpill (exp, [y])
+                   ) handle _ => ToSpill (exp, [y])
+                end
+            | (Alloc(r), env) => 
+                 let val (exp2,env') = g_repeat dest cont env N
+                 in NoSpill(concat exp1 r exp2, env')
+                 end
+     end
 and
-
-g_repeat dest cont regenv exp =                  (*  early spilling *)
-   case g dest cont regenv exp of
-      NoSpill(exp', regenv') => (exp', regenv')
+g_repeat dest cont regenv exp =   (* early spilling *)
+  case g dest cont regenv exp 
+   of NoSpill(exp', regenv') => (exp', regenv')
     | ToSpill(exp, xs) =>
         let val (exp,regenv) = 
-              List.foldl
-               (fn (x,(exp,env)) => save x exp env)
+              List.foldl (fn (x,(exp,env)) => save x exp env)
                (exp, regenv)
                xs
         in
           g_repeat dest cont regenv exp
         end
-
 and
-
 g'_if dest cont regenv exp constr e1 e2 = 
-  let 
-    val (e1', regenv1) = g_repeat dest cont regenv e1
-    val (e2', regenv2) = g_repeat dest cont regenv e2
-    val regenv' = List.foldl (fn ((key,value), m) => M.insert(m,key,value)) regenv1 (M.listItems regenv2)
+ let val (e1', regenv1) = g_repeat dest cont regenv e1
+     val (e2', regenv2) = g_repeat dest cont regenv e2
+     val regenv' = 
+       List.foldl (fn ((key,value), m) => M.insert(m,key,value)) regenv1 
+                  (M.listItems regenv2)
   in
     NoSpill(constr e1' e2', regenv')
   end
+;
 
-(* The following code is needed only for non-SSA expressions 
+(*---------------------------------------------------------------------------
+ The following code is needed only for non-SSA expressions 
     val regenv' =
       List.foldl
       (fn (x,regenv') =>
@@ -422,50 +406,49 @@ g'_if dest cont regenv exp constr e1 e2 =
   in
     case
       List.filter
-      (fn x => not (is_reg x) andalso (M.peek(regenv',x) = NONE) andalso x <> dest)
+      (fn x => not (is_reg x) andalso 
+               (M.peek(regenv',x) = NONE) andalso x <> dest)
       (fv cont)
     of 
       [] => NoSpill(constr e1' e2', regenv')
     | xs => ToSpill(exp, xs)
   end
-*)
+  ---------------------------------------------------------------------------*)
 
 (* --------------------------------------------------------------------*)
 (* Reduce the number of memory slots by reusing memory variables.      *)
 (* The mechanism is similar to that of allocating registers; but we    *)
-(* unlimited number of memory slots.                                   *)
+(* assume an unlimited number of memory slots.                         *)
 (* --------------------------------------------------------------------*)
 
 (* The first available memory slot that doesn't conflict with live "slots" *)
 
 fun first_avail_slot env cont = 
-  let 
-      fun indexOfSlot s = valOf(Int.fromString(String.substring(s, 1, String.size s - 1)))
-
-      val live = List.foldl (fn (t,ts) => 
-			     let val x = M.find(env,t) in 
-				 if is_mem x then x ::ts else ts end handle _ => ts) [] (free_vars cont)
-      val max_slot = indexOfSlot(state(!mStrm))
-      fun candidate i =  (* the first available register *)
+ let fun indexOfSlot s = 
+        valOf(Int.fromString(String.substring(s, 1, String.size s - 1)))
+     val live = List.foldl (fn (t,ts) => 
+			     let val x = M.find(env,t) 
+                             in if is_mem x then x::ts else ts 
+                             end handle _ => ts) [] (free_vars cont)
+     val max_slot = indexOfSlot(state(!mStrm))
+     fun candidate i =  (* the first available register *)
         if i > max_slot then next_mvar()
         else
           let val cur_slot = mk_var("m" ^ Int.toString i, !VarType)
-          in if list_mem cur_slot live then
-	        candidate (i+1)
+          in if Lib.mem cur_slot live then candidate (i+1)
              else cur_slot
           end
-  in
-     candidate 1
-  end
+ in
+    candidate 1
+ end
 
-(* reuse memory slots that will be "live" any more *)
+(* reuse memory slots that will not be "live" any more *)
 
 fun alloc_mem (args,body) =
-  let
-     val body' = rhs (concl (SIMP_CONV bool_ss [ELIM_USELESS_LET] body)) handle _ => body
-     val (save,loc) = (mk_const("save", mk_type("fun",[!VarType, !VarType])),
-		       mk_const("loc", mk_type("fun",[!VarType, !VarType])))
-
+ let val body' = rhs (concl 
+                   (QCONV(SIMP_CONV bool_ss [ELIM_USELESS_LET]) body))
+     val (save,loc) = (mk_const("save", (!VarType) --> (!VarType)),
+		       mk_const("loc", (!VarType) --> (!VarType)))
      fun trav t env cont =
        if is_let t then
            let val (v,M,N) = dest_plet t
@@ -508,10 +491,12 @@ fun alloc_mem (args,body) =
            mk_comb (loc, M.find (env, t) handle _ => t)
        else t
 
-     val memenv = List.foldl (fn (t, m) => if is_mem t then (next_mvar(); M.insert(m,t,t)) else m) 
-	 (M.mkDict tvarOrder) (strip_pair args)
-     fun move_mindex i = if i = M.numItems memenv then () else (next_mvar();move_mindex (i + 1))
-
+     val memenv = List.foldl (fn (t, m) => 
+                    if is_mem t then (next_mvar(); M.insert(m,t,t)) else m) 
+                  (M.mkDict tvarOrder) (strip_pair args)
+     fun move_mindex i = 
+       if i = M.numItems memenv then () 
+       else (next_mvar();move_mindex (i + 1))
   in
      (reset_mvar ();
       move_mindex 0;
@@ -524,76 +509,84 @@ fun alloc_mem (args,body) =
 (* --------------------------------------------------------------------*)
 
 fun parallel_move dst src exp =
-  let
-    fun mk_atom tm = mk_comb (inst [alpha |-> type_of tm] (prim_mk_const{Name="atom",Thy="Normal"}), tm)
-
-    val sane = ref true
-    val (dstL, srcL) = (strip_pair dst, strip_pair src)
-    val spotL = !regL @ #1 (List.foldl (fn (_,(l,i)) => 
-         (l @ [mk_var("m" ^ Int.toString i, !VarType)], i+1)) ([],1) (hd srcL :: srcL))
-    fun get_avail_spot l = 
+ let val sane = ref true
+   val (dstL, srcL) = (strip_pair dst, strip_pair src)
+   val (tmpL,_) = List.foldl (fn (_,(l,i)) => 
+                                (l @ [mk_var("m" ^ Int.toString i, !VarType)],
+                                 i+1)) 
+                    ([],1) (hd srcL :: srcL)
+   val spotL = !regL @ tmpL 
+   fun get_avail_spot l = 
         let val l' = l @ free_vars exp
-        in valOf (List.find (fn x => List.all (fn y => not (x = y)) l') spotL)
+        in valOf (List.find (fn x => List.all (not o equal x) l') spotL)
         end
 
-    val transfer_r = let val r = get_avail_spot (srcL @ dstL) in
-                  if is_mem r then hd spotL 
-                  else r
-                end
+   val transfer_r = 
+      let val r = get_avail_spot (srcL @ dstL) 
+      in if is_mem r then hd spotL else r
+      end
 
-    fun move (d,s,r) t =
-        if is_mem s andalso is_mem d then
-          let val real_r = if is_mem r then (sane := false; transfer_r) else r in
+   fun move (d,s,r) t =
+    if is_mem s andalso is_mem d 
+    then let val real_r = 
+               if is_mem r then (sane := false; transfer_r) else r 
+         in
             mk_plet(real_r, mk_atom s, mk_plet(d, mk_atom real_r, t))
-          end
-        else
-          mk_plet(d, mk_atom s, t)
+         end
+    else mk_plet(d, mk_atom s, t)
 
-    fun moves (t,[],[]) = t
-     |  moves (t, d::dL, s::sL) = 
-          if d = s then t
-          else
-            if List.exists (curry (op =) d) sL then (* d is still live *)
-              let val spot = get_avail_spot (d :: s :: sL)
-                  val transfer_r = get_avail_spot (spot :: d :: s :: sL)
-                  val t' = move(d,s,transfer_r) (moves(t, dL, 
-                     List.map (fn x => if x = d then spot else if x = s then d else x) sL))
-              in
-                move (spot,d, transfer_r) t' (* d is stored in spot in the beginning *)
-              end
-            else
-              move(d,s,get_avail_spot (d :: s :: sL)) (moves(t, dL, List.map (fn x => if x = s then d else x) sL))
-
-     val exp' = if !sane then moves(exp, dstL, srcL)
-             else
-               (* store the value of the trasfterring register into memory if needed *)
-               let val tmp_m = valOf (List.find (fn x => is_mem x andalso 
-                        List.all (fn y => not (x = y)) (srcL @ dstL)) spotL) in
-                 mk_plet(transfer_r, mk_atom tmp_m,      (* load the transferring register *)
-                   moves(mk_plet(tmp_m, mk_atom transfer_r, exp), dstL, srcL)) (* store the transferring register *)
+   fun moves (t,[],[]) = t
+     | moves (t, d::dL, s::sL) = 
+         if d = s then t
+         else
+          if List.exists (equal d) sL (* d is still live *)
+          then let val spot = get_avail_spot (d :: s :: sL)
+                   val transfer_r = get_avail_spot (spot :: d :: s :: sL)
+                   val tmp = List.map 
+                              (fn x => if x = d then spot else 
+                                       if x = s then d else x) 
+                              sL
+                   val t' = move (d,s,transfer_r) (moves(t, dL, tmp))
+               in (* d is stored in spot in the beginning *)
+                 move (spot,d, transfer_r) t' 
                end
-  in
+          else
+             move(d,s,get_avail_spot (d :: s :: sL))
+                 (moves(t, dL, List.map (fn x => if x = s then d else x) sL))
+   val exp' = 
+     if !sane then moves(exp, dstL, srcL)
+     else (* store value of transferring register in memory if needed *)
+       let val sdL = srcL @ dstL
+           val opt = List.find (fn x => is_mem x andalso 
+                                        List.all (not o equal x) sdL) spotL
+           val tmp_m = valOf opt
+       in (* load the transferring register *)
+          mk_plet(transfer_r, mk_atom tmp_m,      
+                  moves(mk_plet(tmp_m, mk_atom transfer_r, exp), dstL, srcL))
+                    (* store the transferring register *)
+       end
+ in
     exp'
-  end
+ end
 
 fun refine_tail_recursion def =
-  let
-    val (fname, fbody) = dest_eq (concl def)
-    val (args,body) = dest_pabs fbody
-    val lem = if is_let body then CONV_RULE (RHS_CONV (SIMP_CONV pure_ss [Once LET_THM])) def
+ let val (fname, fbody) = dest_eq (concl def)
+   val (args,body) = dest_pabs fbody
+   val lem = if is_let body 
+              then CONV_RULE (RHS_CONV(SIMP_CONV pure_ss [Once LET_THM])) def
               else def
-    val body = #2 (dest_pabs (rhs (concl lem))) 
-    val is_recursive = (find_term (curry (op =) fname) body; true) handle _ => false
-    val lems = ref []
-  in
-    if not is_recursive then def
-    else
-      let
-        fun trav t =
+   val body = #2 (dest_pabs (rhs (concl lem))) 
+   val is_recursive = Lib.can (find_term (equal fname)) body
+   val lems = ref []
+ in
+   if not is_recursive then def else
+   let fun trav t =
           if is_let t then
             let val (v,M,N) = dest_plet t
             in if is_comb M andalso #1(strip_comb M) = fname then
-                 let val _ = lems := PBETA_RULE (SIMP_CONV bool_ss [Once LET_THM] t) :: !lems
+                 let val _ = lems := PBETA_RULE 
+                                       (SIMP_CONV bool_ss [Once LET_THM] t) 
+                                     :: !lems
                      val src = #2(dest_comb M)
                      val exp = subst [src |-> args] (subst [v |-> M] N)
                  in
@@ -623,73 +616,77 @@ fun refine_tail_recursion def =
         val th = prove(mk_eq(fname, mk_pabs(args,body')),
                    REWRITE_TAC [Once lem] THEN
                    SIMP_TAC bool_ss ([FUN_EQ_THM, LET_ATOM, ATOM_ID] @ (!lems))
-                 ) handle _ => (print "fail to convert a tail recursion into the expected format!"; def)
-      in
-        REWRITE_RULE [ATOM_ID] th
-      end
-  end
+                 ) handle _ => 
+           (print "failed to convert a tail recursion into expected format!"; 
+            def)
+   in
+      REWRITE_RULE [ATOM_ID] th
+   end
+ end
 
 (* --------------------------------------------------------------------*)
 (* Register Allocation                                                 *)
 (* --------------------------------------------------------------------*)
 
-fun reset () = 
-  (regL := mk_regs();
-   reset_mvar();
-   reset_tvar()
-  )
+fun reset () = (regL := mk_regs(); reset_mvar(); reset_tvar() );
 
-(* Assign registers to inputs; memory slots will be used when there are too many paramenters *)
+(*---------------------------------------------------------------------------*)
+(* Assign registers to inputs; memory slots will be used when there are too  *)
+(* many paramenters                                                          *)
+(*---------------------------------------------------------------------------*)
 
 fun args_env args = 
-   let val argL = strip_pair args
-       fun assgn_v (v,(i,regenv)) = 
-            (i+1, M.insert (regenv, v, 
-		if i < !numRegs then mk_var ("r" ^ Int.toString i, !VarType)
-                else next_mvar()))
+ let val argL = strip_pair args
+     fun assgn_v (v,(i,regenv)) = 
+       (i+1, 
+        M.insert (regenv, v, 
+                  if i < !numRegs then mk_var ("r" ^ Int.toString i, !VarType)
+                  else next_mvar()))
    in
        #2 (List.foldl assgn_v (0, M.mkDict tvarOrder) argL)
    end
 
-(* step1: configurate the environment;
-   step2: obtain a allocation scheme by term rewriting;
-   step3: prove the correctness of the scheme by showing the result is alpha-equivalent to the source program
-*)
+(*---------------------------------------------------------------------------*)
+(* step1: configure the environment;                                         *)
+(* step2: obtain an allocation scheme by term rewriting;                     *)
+(* step3: prove the correctness of the scheme by showing the result is       *)
+(* alpha-equivalent to the source program.                                   *)
+(*---------------------------------------------------------------------------*)
 
 fun reg_alloc def =
-  let
-    val (fname, fbody) = dest_eq (concl def)
-    val (args,body) = dest_pabs fbody
-    val (sane,var_type) = pre_check(args,body)
-  in
-    if sane then
-      let (* set the variable type according to the given program *)
-    	val _ = (VarType := var_type; reset())
-    	val regenv = args_env args
-    	val args1 = subst (tuple_subst_rules (strip_pair args) regenv) args
-    	val dest = hd (!regL); (* assgn_exp (last_exp body) *)
-    	val cont = dest
-    	val body1 = #1 (g_repeat dest cont regenv body)
-    	val body2 = alloc_mem(args1,body1)
+ let
+   val (fname, fbody) = dest_eq (concl def)
+   val (args,body) = dest_pabs fbody
+   val (sane,var_type) = pre_check(args,body)
+ in
+  if sane then
+   let (* set the variable type according to the given program *)
+      val _ = (VarType := var_type; reset())
+      val regenv = args_env args
+      val args1 = subst (tuple_subst_rules (strip_pair args) regenv) args
+      val dest = hd (!regL)
+      val cont = dest
+      val body1 = #1 (g_repeat dest cont regenv body)
+      val body2 = alloc_mem(args1,body1)
+      val tha = QCONV(SIMP_CONV pure_ss [LET_SAVE, LET_LOC, loc_def]) body2
+      val th1 = SYM (PBETA_RULE tha)
+      val body3 = lhs (concl th1)
+      val th2 = ALPHA fbody (mk_pabs (args1,body3)) handle e 
+                  => (print "the allocation is incomplete or incorrect"; 
+                      Raise e)
+      val th3 = CONV_RULE (RHS_CONV (ONCE_REWRITE_CONV [th1])) th2
+      val th4 = TRANS def th3
+      val th5 = (BETA_RULE o REWRITE_RULE [save_def, loc_def]) th4
+      val th6 = refine_tail_recursion th5
+   in
+     th6
+   end
+  else
+   ( print("The source program is invalid!\ 
+         \ (e.g. all variables are not of the same type)");
+     def
+   )
+  end;
 
-    	val th1 = GSYM (PBETA_RULE (SIMP_CONV pure_ss [LET_SAVE, LET_LOC, loc_def] body2))
-            handle _ => REFL body2
-    	val body3 = lhs (concl (th1))
-    	val th2 = ALPHA fbody (mk_pabs (args1,body3))
-		  handle e => (print "the allocation is incomplete or incorrect"; Raise e)
-    	val th3 = CONV_RULE (RHS_CONV (ONCE_REWRITE_CONV [th1])) th2
-    	val th4 = TRANS def th3
-    	val th5 = (BETA_RULE o REWRITE_RULE [save_def, loc_def]) th4
-        val th6 = refine_tail_recursion th5
-      in
-    	th6
-      end
-    else
-     ( print("The source program is invalid! (e.g. all variables are not of the same type)");
-       def
-     )
-  end
-
-(* --------------------------------------------------------------------*)
 
 end
